Try starting proof of 2nd part of equivalence

warblreequiv/RegexpTranslation.v
@@ -1,13 +1,26 @@
-From Warblre Require Import Patterns.
+From Warblre Require Import Patterns Result Errors Coercions Notation Base.
 From Linden Require Import Regex CharsWarblre LindenParameters.
+Import Notation.
+Import Result.
+Import Result.Notations.
+Local Open Scope result_flow.
 
-
-Fixpoint to_warblre_regex (r: regex) :=
+Fixpoint to_warblre_regex (r: regex): Result Patterns.Regex CompileError :=
   match r with
-  | Epsilon => Patterns.Empty
+  | Epsilon => Success Patterns.Empty
   | Character cd => char_descr_to_regex cd
-  | Disjunction r1 r2 => Patterns.Disjunction (to_warblre_regex r1) (to_warblre_regex r2)
-  | Sequence r1 r2 => Patterns.Seq (to_warblre_regex r1) (to_warblre_regex r2)
-  | Star greedy r1 => Patterns.Quantified (to_warblre_regex r1) (if greedy then Patterns.Greedy Patterns.Star else Patterns.Lazy Patterns.Star)
-  | Group id r => Patterns.Group None (to_warblre_regex r)
+  | Disjunction r1 r2 =>
+    let! wr1 =<< to_warblre_regex r1 in
+    let! wr2 =<< to_warblre_regex r2 in
+    Success (Patterns.Disjunction wr1 wr2)
+  | Sequence r1 r2 =>
+    let! wr1 =<< to_warblre_regex r1 in
+    let! wr2 =<< to_warblre_regex r2 in
+    Success (Patterns.Seq wr1 wr2)
+  | Star greedy r1 =>
+    let! wr1 =<< to_warblre_regex r1 in
+    Success (Patterns.Quantified wr1 (if greedy then Patterns.Greedy Patterns.Star else Patterns.Lazy Patterns.Star))
+  | Group id r =>
+    let! wr =<< to_warblre_regex r in
+    Success (Patterns.Group None wr)
   end.
