warblreequiv/LWEquivTree.v
@@ -1,0 +1,64 @@
+From Coq Require Import PeanoNat ZArith Bool Lia Program.Equality List Program.Wf.
+From Linden Require Import Tree LindenParameters CharsWarblre TMatching Chars Regex Semantics RegexpTranslation.
+From Warblre Require Import Patterns Result Notation Errors Node RegExpRecord Base Coercions Semantics Typeclasses.
+Import Patterns.
+Import Result.Result.
+Import Result.Notations.
+Import Result.Notations.Boolean.
+Import Coercions.
+Import Notation.
+
+Local Open Scope result_flow.
+
+(*Definition state_of_input (inp: input) : MatchState :=
+    let '(Input next pref) := inp in
+    let end_ind := List.length pref in
+    let s := List.rev pref ++ next in
+    {|
+        MatchState.input := s;
+        MatchState.endIndex := Z.of_nat end_ind;
+        MatchState.captures := nil
+    |}.*)
+
+Inductive ms_matches_inp: MatchState -> input -> Prop :=
+| Ms_matches_inp: forall (s: string) (end_ind: nat) cap (next pref: string),
+    List.length pref = end_ind -> List.rev pref ++ next = s ->
+    ms_matches_inp {| MatchState.input := s; MatchState.endIndex := Z.of_nat end_ind;
+        MatchState.captures := cap |} (Input next pref).
+
+Definition tMC_is_tree (tmc: TMatcherContinuation) (reg: regex) (cont: continuation) (inp: input) :=
+    forall s, ms_matches_inp s inp -> match tmc s with
+    | Error _ => True (* finer modeling? *)
+    | Success t => is_tree reg cont inp t
+    end.
+
+Section Main.
+  Context (s0: string).
+
+  Inductive input_compat: input -> Prop :=
+  | Input_compat: forall next pref, List.rev pref ++ next = s0 -> input_compat (Input next pref).
+
+  Theorem tmatcher_bt: forall reg ctx rer,
+    let wreg' := to_warblre_regex reg in
+    match wreg' with
+    | Error _ => True
+    | Success wreg =>
+      match tCompileSubPattern wreg ctx rer forward with
+      | Error _ => True
+      | Success tm => forall (tmc: TMatcherContinuation) (regc: regex) (cont: continuation),
+        (forall inp, input_compat inp -> tMC_is_tree tmc regc cont inp) ->
+        forall inp, input_compat inp -> tMC_is_tree (fun s => tm s tmc) reg (Areg regc::cont) inp
+      end
+    end.
+  Proof.
+    intros reg ctx rer.
+    revert ctx.
+    induction reg.
+    - simpl. intros _.
+      intros.
+      intro. intro.
+      specialize (H inp H0 s H1).
+      destruct (tmc s) eqn:?; simpl; try exact I.
+      apply tree_pop_reg. assumption.
+    - simpl.
+      
