warblreequiv/TMatching.v
@@ -285,269 +285,32 @@ match self with
 | _ => Error CompileError.AssertionFailed
 end.
 
-Inductive tree_res'_error :=
-  | MismatchingTree.
+(** >>
+    22.2.2.2 Runtime Semantics: CompilePattern
 
-Instance tree_res'_error_assert: AssertionError tree_res'_error := {| Result.f := MismatchingTree |}.
-
-Definition advance_ms (s: MatchState): MatchState :=
-  {|
-    MatchState.input := MatchState.input s;
-    MatchState.endIndex := (MatchState.endIndex s + 1)%Z;
-    MatchState.captures := MatchState.captures s |}.
-
-Fixpoint reset_groups_ms (gidl: list Groups.group_id) (s: MatchState): Result MatchState tree_res'_error :=
-  let '(match_state inp endInd cap) := s in
-  match gidl with
-  | nil => Success s
-  | x::q =>
-    set cap[x] := None in
-    reset_groups_ms q (match_state inp endInd cap)
-  end.
-
-(* A list of currently open groups *)
-Definition open_groups := list (Groups.group_id * integer).
-
-Fixpoint has_group (id: Groups.group_id) (gl: open_groups): bool :=
-  match gl with
-  | nil => false
-  | (id', _)::q => if id == id' then true else has_group id q
-  end.
-
-Fixpoint close_group (id: Groups.group_id) (gl: open_groups) end_index: Result (CaptureRange * open_groups) tree_res'_error :=
-  match gl with
-  | nil => Error MismatchingTree
-  | (id', start)::q =>
-    if id == id' then
-      Success (capture_range start end_index, q)
-    else
-      let! (range, q') =<< close_group id q end_index in
-      Success (range, (id', start)::q')
-  end.
-
-(* TODO Direction *)
-Definition group_effect' (g: groupaction) (s: MatchState) (gl: open_groups): Result (MatchState * open_groups) tree_res'_error :=
-  match g with
-  | Open gid =>
-      Success (s, (gid, MatchState.endIndex s)::gl)
-  | Close gid =>
-      let cap := MatchState.captures s in
-      let! (range, gl') =<< close_group gid gl (MatchState.endIndex s) in
-      set cap[gid] := range in
-      Success (match_state (MatchState.input s) (MatchState.endIndex s) cap, gl')
-  | Reset gidl =>
-      let! s' =<< reset_groups_ms gidl s in
-      Success (s', gl)
-  end.
-
-(* returning the highest-priority result *)
-(* we also return the corresponding state *)
-(* TODO Direction *)
-Fixpoint tree_res' (t:tree) (s: MatchState) (gl: open_groups): Result (option MatchState) tree_res'_error :=
-  match t with
-  | Mismatch => Success None
-  | Match => Success (Some s)
-  | Choice t1 t2 =>
-      let! res1 =<< tree_res' t1 s gl in
-      match res1 with
-      | None => tree_res' t2 s gl
-      | Some _ => Success res1
-      end
-  | Read c t1 => 
-    if List.nth (Z.to_nat (MatchState.endIndex s)) (MatchState.input s) c == c then
-      tree_res' t1 (advance_ms s) gl
-    else
-      Error MismatchingTree
-  | CheckFail _ => Success None
-  | CheckPass _ t1 => tree_res' t1 s gl
-  | GroupAction g t1 => 
-    let! (s', gl') =<< group_effect' g s gl in tree_res' t1 s' gl'
-  end.
-
-
-Definition equiv_tree (mc: MatcherContinuation) (tmc: TMatcherContinuation) (gl: open_groups) :=
-  forall s: MatchState, 
-  match tmc s, mc s with
-  | Error _, _ | _, Error _ => True (* finer modeling? *)
-  | Success t, Success res => tree_res' t s gl = Success res
-  end.
-
-Definition id_mcont: MatcherContinuation := fun x => Success (Some x).
-Definition id_tmcont: TMatcherContinuation := fun _ => Success Match.
-
-Lemma id_equiv: equiv_tree id_mcont id_tmcont nil.
-Proof.
-  intro s. simpl. reflexivity.
-Qed.
-
-
-Theorem compile_tcompile: forall reg ctx rer,
-  let m' := Semantics.compileSubPattern reg ctx rer forward in
-  let tm' := tCompileSubPattern reg ctx rer forward in
-  match m', tm' with
-  | Error _, _ | _, Error _ => True
-  | Success m, Success tm =>
-  forall mc tmc gl, equiv_tree mc tmc gl -> equiv_tree (fun s => m s mc) (fun s => tm s tmc) gl
-  end.
-Proof.
-  intros reg ctx rer.
-  revert ctx.
-  induction reg; simpl.
-  - (* Empty *)
-    intros. unfold equiv_tree in *. assumption.
-  - (* Character *)
-    intros. unfold equiv_tree in *. intro.
-    unfold tCharacterSetMatcher, Semantics.characterSetMatcher.
-    simpl.
-    remember ((_ <? 0)%Z || _) as b.
-    destruct b.
-    + simpl. reflexivity.
-    + remember (Z.min _ _) as index.
-      remember (List.List.Indexing.Int.indexing _ _) as chr'.
-      destruct chr'; simpl; try (exact I).
-      remember (if CharSet.exist_canonicalized _ _ _ then false else true) as b2.
-      destruct b2; simpl.
-      1: reflexivity.
-      remember (match_state _ _ _) as s'.
-      specialize (H s').
-      destruct (tmc s'); simpl; try exact I.
-      destruct (mc s'); simpl; try exact I.
-      replace (Z.min (MatchState.endIndex s) (MatchState.endIndex s + 1)) with (MatchState.endIndex s) in Heqindex by lia.
-      rewrite Heqindex in Heqchr'.
-      replace (nth _ _ s0) with s0 by admit.
-      rewrite EqDec.reflb.
-      rewrite <- H.
-      f_equal.
-      unfold advance_ms.
-      rewrite Heqs'.
-      reflexivity.
-  - (* Dot; mostly same as character *)
-    intros.
-    intro s.
-    unfold tCharacterSetMatcher, Semantics.characterSetMatcher.
-    simpl.
-    remember ((_ <? 0)%Z || _) as b.
-    destruct b.
-    + simpl. reflexivity.
-    + remember (Z.min _ _) as index.
-      remember (List.List.Indexing.Int.indexing _ _) as chr'.
-      destruct chr'; simpl; try (exact I).
-      remember (if CharSet.exist_canonicalized _ _ _ then false else true) as b2.
-      destruct b2; simpl.
-      1: reflexivity.
-      remember (match_state _ _ _) as s'.
-      specialize (H s').
-      destruct (tmc s'); simpl; try exact I.
-      destruct (mc s'); simpl; try exact I.
-      replace (Z.min (MatchState.endIndex s) (MatchState.endIndex s + 1)) with (MatchState.endIndex s) in Heqindex by lia.
-      rewrite Heqindex in Heqchr'.
-      replace (nth _ _ s0) with s0 by admit.
-      rewrite EqDec.reflb.
-      rewrite <- H.
-      f_equal.
-      unfold advance_ms.
-      rewrite Heqs'.
-      reflexivity.
-  - (* Unsupported case *)
-    intro. destruct (match ae with | DecimalEsc de => _ | ACharacterClassEsc cce => _ | ACharacterEsc ce => _ | GroupEsc gn => _ end); split.
-  - (* Character class: unsupported *)
-    intro. destruct (let! _ =<< _ in _); split.
-  - (* Disjunction *)
-    intro.
-    remember (Disjunction_left reg2 :: ctx) as ctxleft.
-    remember (Disjunction_right reg1 :: ctx) as ctxright.
-    specialize (IHreg1 ctxleft).
-    specialize (IHreg2 ctxright).
-    destruct (Semantics.compileSubPattern reg1 _ _ _) as [m1|] eqn:?; simpl; try exact I.
-    destruct (Semantics.compileSubPattern reg2 _ _ _) as [m2|] eqn:?; simpl; try exact I.
-    destruct (tCompileSubPattern reg1 _ _ _) as [tm1|] eqn:?; simpl; try exact I.
-    destruct (tCompileSubPattern reg2 _ _ _) as [tm2|] eqn:?; simpl; try exact I.
-    simpl in *.
-    intros.
-    intro s'.
-    specialize (IHreg1 mc tmc gl H s').
-    specialize (IHreg2 mc tmc gl H s').
-    simpl in *.
-    destruct (tm1 s' tmc) as [t1|] eqn:?; simpl; try exact I.
-    destruct (tm2 s' tmc) as [t2|] eqn:?; simpl; try exact I.
-    destruct (m1 s' mc) as [r|] eqn:?; simpl; try exact I.
-    destruct r eqn:?; simpl.
-    + rewrite IHreg1. simpl. reflexivity.
-    + destruct (m2 s' mc) as [r2|] eqn:?; simpl; try exact I.
-      rewrite IHreg1. simpl. assumption.
-  - (* Quantifier *)
-    intro.
-    admit.
-  - (* Sequence *)
-    intro.
-    remember (Seq_left reg2 :: ctx) as ctxleft.
-    remember (Seq_right reg1 :: ctx) as ctxright.
-    specialize (IHreg1 ctxleft).
-    specialize (IHreg2 ctxright).
-    destruct (Semantics.compileSubPattern reg1 _ _ _) as [m1|] eqn:?; simpl; try exact I.
-    destruct (Semantics.compileSubPattern reg2 _ _ _) as [m2|] eqn:?; simpl; try exact I.
-    destruct (tCompileSubPattern reg1 _ _ _) as [tm1|] eqn:?; simpl; try exact I.
-    destruct (tCompileSubPattern reg2 _ _ _) as [tm2|] eqn:?; simpl; try exact I.
-    simpl in *.
-    intros. intro.
-    specialize (IHreg2 mc tmc gl H).
-    specialize (IHreg1 (fun s0 => m2 s0 mc) (fun s0 => tm2 s0 tmc) gl IHreg2 s).
-    simpl in *.
-    assumption.
-  - (* Group *)
-    intro.
-    remember (Group_inner name :: ctx) as ctx'.
-    specialize (IHreg ctx').
-    destruct (Semantics.compileSubPattern reg ctx' rer forward) as [m|] eqn:?; simpl; try exact I.
-    destruct (tCompileSubPattern reg ctx' rer forward) as [tm|] eqn:?; simpl; try exact I.
-    intros mc tmc gl H s.
-    simpl in *.
-    remember (fun y : MatchState => _) as treecont.
-    remember (fun y : MatchState => let! r =<< _ in let! cap =<< _ in mc _) as origcont.
-    remember (StaticSemantics.countLeftCapturingParensBefore _ ctx + 1) as gid.
-    set (gl' := (gid, MatchState.endIndex s)::gl).
-    specialize (IHreg origcont treecont gl').
-    assert (equiv_tree origcont treecont gl') as Hequivcont.
-    {
-      intro y.
-      rewrite Heqtreecont, Heqorigcont.
-      remember (MatchState.endIndex s) as x.
-      destruct negb eqn:?; simpl; try exact I.
-      destruct (gid =? 0) eqn:?; simpl; try exact I.
-      destruct List.List.Update.Nat.One.update eqn:?; simpl; try exact I.
-      remember (match_state _ _ s0) as s'.
-      destruct (tmc s') as [t|] eqn:?; simpl; try exact I.
-      destruct (mc s') as [res|] eqn:?; simpl; try exact I.
-      rewrite EqDec.reflb. simpl.
-      rewrite Heqb0.
-      (* Prove: the result of List.List.....Update does not depend on the type of the error that should be returned if any *)
-      replace (@List.List.Update.Nat.One.update _ tree_res'_error _ _ _ (gid - 1)) with (@Success _ tree_res'_error s0) by admit.
-      simpl.
-      specialize (H s').
-      rewrite Heqt, Heqm0 in H.
-      rewrite Heqs' in H.
-      (* mismatching inputs... but all the match states that we manipulate here use the same input, morally *)
-      admit.
-    }
-    specialize (IHreg Hequivcont s).
-    simpl in *.
-    destruct (tm s treecont) as [t|] eqn:?; simpl; try exact I.
-    destruct (m s origcont) as [res|] eqn:?; simpl; try exact I.
-    assumption.
-  - (* Unsupported *)
-    split.
-  - (* Unsupported *)
-    split.
-  - (* Unsupported *)
-    split.
-  - (* Unsupported *)
-    split.
-  - (* Lookahead: unsupported *)
-    intro. destruct (let! _ =<< _ in _); split.
-  - (* Negative lookahead: unsupported *)
-    intro. destruct (let! _ =<< _ in _); split.
-  - (* Lookbehind: unsupported *)
-    intro. destruct (let! _ =<< _ in _); split.
-  - (* Negative lookbehind: unsupported *)
-    intro. destruct (let! _ =<< _ in _); split.
-Admitted.
+    The syntax-directed operation CompilePattern takes argument rer (a RegExp Record) and returns an Abstract Closure
+    that takes a List of characters and a non-negative integer and returns a MatchResult.
+    It is defined piecewise over the following productions:
+<<*)
+(** >>  Pattern :: Disjunction <<*)
+Definition tCompilePattern (r: Regex) (rer: RegExpRecord): Result (list Character -> non_neg_integer -> TMatchResult) CompileError :=
+  (*>> 1. Let m be CompileSubpattern of Disjunction with arguments rer and forward. <<*)
+  let! m =<< tCompileSubPattern r nil rer forward in
+  (*>> 2. Return a new Abstract Closure with parameters (Input, index) that captures rer and m and performs the following steps when called: <<*)
+  Success (fun (input: list Character) (index: non_neg_integer) =>
+    (*>> a. Assert: Input is a List of characters. <<*)
+    (*>> b. Assert: 0 ≤ index ≤ the number of elements in Input. <<*)
+    assert! (0 <=? index)%nat && (index <=? (length input))%nat ;
+    (*>> c. Let c be a new MatcherContinuation with parameters (y) that captures nothing and performs the following steps when called: <<*)
+    let c: TMatcherContinuation := fun (y: MatchState) =>
+      (*>> i. Assert: y is a MatchState. <<*)
+      (*>> ii. Return y. <<*)
+      Success Match
+    in
+    (*>> d. Let cap be a List of rer.[[CapturingGroupsCount]] undefined values, indexed 1 through rer.[[CapturingGroupsCount]]. <<*)
+    (* + The fact that the array starts at 1 is handled by the nat indexer +*)
+    let cap := List.repeat undefined (RegExpRecord.capturingGroupsCount rer) in
+    (*>> e. Let x be the MatchState (Input, index, cap). <<*)
+    let x := match_state input (Z.of_nat index) cap in
+    (*>> f. Return m(x, c). <<*)
+    m x c).
